Lean/Egg/Core/Explanation/Expr.lean
@@ -15,41 +15,41 @@ where
   coord (g : Expr → Expr → MetaM (Expr × Expr × ζ)) (c : Nat) (e₁ e₂ : Expr) : MetaM (Expr × Expr × ζ) := do
     match c, e₁, e₂ with
     | 0, .app f₁ a₁, .app f₂ a₂ => do
-      unless ← isDefEq a₁ a₂ do throwDifferent e₁ e₂
+      unless ← (return a₁ == a₂) <||> isDefEq a₁ a₂ do throwDifferent e₁ e₂
       let (f₁', f₂', z) ← g f₁ f₂
       return (.app f₁' a₁, .app f₂' a₂, z)
     | 1, .app f₁ a₁, .app f₂ a₂ => do
-      unless ← isDefEq f₁ f₂ do throwDifferent e₁ e₂
+      unless ← (return f₁ == f₂) <||> isDefEq f₁ f₂ do throwDifferent e₁ e₂
       let (a₁', a₂', z) ← g a₁ a₂
       return (.app f₁ a₁', .app f₂ a₂', z)
     | 0, .lam n₁ t₁ b₁ i₁, .lam n₂ t₂ b₂ i₂ => do
-      unless ← isDefEq b₁ b₂ do throwDifferent e₁ e₂
+      unless ← (return b₁ == b₂) <||> isDefEq b₁ b₂ do throwDifferent e₁ e₂
       let (t₁', t₂', z) ← g t₁ t₂
       return (.lam n₁ t₁' b₁ i₁, .lam n₂ t₂' b₂ i₂, z)
     | 1, .lam n₁ t₁ b₁ i₁, .lam _ t₂ b₂ _ => do
-      unless ← isDefEq t₁ t₂ do throwDifferent e₁ e₂
+      unless ← (return t₁ == t₂) <||> isDefEq t₁ t₂ do throwDifferent e₁ e₂
       withLocalDecl n₁ i₁ t₁ fun fvar => do
         let (b₁', b₂', z) ← g (b₁.instantiateRev #[fvar]) (b₂.instantiateRev #[fvar])
         return (← mkLambdaFVars #[fvar] b₁', ← mkLambdaFVars #[fvar] b₂', z)
     | 0, .forallE n₁ t₁ b₁ i₁, .forallE n₂ t₂ b₂ i₂ => do
-      unless ← isDefEq b₁ b₂ do throwDifferent e₁ e₂
+      unless ← (return b₁ == b₂) <||> isDefEq b₁ b₂ do throwDifferent e₁ e₂
       let (t₁', t₂', z) ← g t₁ t₂
       return (.forallE n₁ t₁' b₁ i₁, .forallE n₂ t₂' b₂ i₂, z)
     | 1, .forallE n₁ t₁ b₁ i₁, .forallE _ t₂ b₂ _ => do
-      unless ← isDefEq t₁ t₂ do throwDifferent e₁ e₂
+      unless ← (return t₁ == t₂) <||> isDefEq t₁ t₂ do throwDifferent e₁ e₂
       withLocalDecl n₁ i₁ t₁ fun fvar => do
         let (b₁', b₂', z) ← g (b₁.instantiateRev #[fvar]) (b₂.instantiateRev #[fvar])
         return (← mkForallFVars #[fvar] b₁', ← mkForallFVars #[fvar] b₂', z)
     | 0, .letE n₁ t₁ v₁ b₁ f₁, .letE n₂ t₂ v₂ b₂ f₂ => do
-      unless ← isDefEq v₁ v₂ <&&> isDefEq b₁ b₂ do throwDifferent e₁ e₂
+      unless ← ((return v₁ == v₂) <||> isDefEq v₁ v₂) <&&> ((return b₁ == b₂) <||> isDefEq b₁ b₂) do throwDifferent e₁ e₂
       let (t₁', t₂', z) ← g t₁ t₂
       return (.letE n₁ t₁' v₁ b₁ f₁, .letE n₂ t₂' v₂ b₂ f₂, z)
     | 1, .letE n₁ t₁ v₁ b₁ f₁, .letE n₂ t₂ v₂ b₂ f₂ => do
-      unless ← isDefEq t₁ t₂ <&&> isDefEq b₁ b₂ do throwDifferent e₁ e₂
+      unless ← ((return t₁ == t₂) <||> isDefEq t₁ t₂) <&&> ((return b₁ == b₂) <||> isDefEq b₁ b₂) do throwDifferent e₁ e₂
       let (v₁', v₂', z) ← g v₁ v₂
       return (.letE n₁ t₁ v₁' b₁ f₁, .letE n₂ t₂ v₂' b₂ f₂, z)
     | 2, .letE n₁ t₁ v₁ b₁ _, .letE _ t₂ v₂ b₂ _ => do
-      unless ← isDefEq t₁ t₂ <&&> isDefEq v₁ v₂ do throwDifferent e₁ e₂
+      unless ← ((return t₁ == t₂) <||> isDefEq t₁ t₂) <&&> ((return v₁ == v₂) <||> isDefEq v₁ v₂) do throwDifferent e₁ e₂
       withLetDecl n₁ t₁ v₁ fun fvar => do
         let (b₁', b₂', z) ← g (b₁.instantiateRev #[fvar]) (b₂.instantiateRev #[fvar])
         return (← mkLetFVars #[fvar] b₁', ← mkLetFVars #[fvar] b₂', z)
