Lean/Egg/Tests/Rudi Groups.lean
@@ -29,6 +29,8 @@ macro "rudify " lhs:term:51 " = " rhs:term : term => `(
   (fun (x : G → G) (_ : α) => x) (fun _ => $rhs)
 )
 
+set_option egg.timeLimit 5
+
 theorem inv_mul_cancel_left : a⁻¹ * (a * b) = b := by group
 
 theorem inv_mul_cancel_left' : rudify a⁻¹ * (a * b) = b := by group
